Soundness.v
@@ -8,6 +8,26 @@ From Elo Require Import Core.
 From Elo Require Import Access.
 From Elo Require Import References.
 
+Local Lemma safe_preserves_inclusion : forall Gamma Gamma',
+  Gamma includes Gamma' ->
+  (safe Gamma) includes (safe Gamma').
+Proof.
+  unfold Map.includes', safe. intros * H *.
+  destruct (Gamma k) eqn:E1; destruct (Gamma' k) eqn:E2;
+  solve [ intros F; inversion F
+        | eapply H in E2; rewrite E1 in E2; inversion E2; subst; trivial
+        ].
+Qed.
+
+Local Lemma update_safe_includes_safe_update : forall Gamma k T,
+  (safe Gamma)[k <== T] includes (safe Gamma[k <== T]).
+Proof.
+  intros ? ? ? k' ? H. unfold safe in H. 
+  destruct (String.string_dec k k'); subst.
+  - rewrite lookup_update_eq in *. destruct T; inversion H; subst; trivial.
+  - rewrite lookup_update_neq in *; trivial.
+Qed.
+
 Local Lemma context_weakening : forall Gamma Gamma' t T,
   Gamma' |-- t is T ->
   Gamma includes Gamma' ->
@@ -15,7 +35,8 @@ Local Lemma context_weakening : forall Gamma Gamma' t T,
 Proof.
   intros. generalize dependent Gamma.
   induction_type; intros;
-  eauto using well_typed_term, update_preserves_inclusion.
+  eauto using well_typed_term, update_preserves_inclusion,
+    safe_preserves_inclusion.
 Qed.
 
 Local Lemma context_weakening_empty : forall Gamma t T,
@@ -40,7 +61,8 @@ Proof.
     try (destruct String.string_dec);
     inversion Htype; subst; 
     eauto using well_typed_term, context_weakening, context_weakening_empty,
-      update_overwrite, update_permutation.
+      update_overwrite, update_permutation,
+      update_safe_includes_safe_update.
   }
   intros * ?. inversion_type. intros. eauto.
 Qed.
